Semantics/FlatMap.v
@@ -1,0 +1,221 @@
+From Stdlib Require Import List.
+Import ListNotations.
+
+From Linden Require Import Tree Semantics Chars Regex.
+From Linden Require Import Parameters.
+From Warblre Require Import Base RegExpRecord.
+
+
+(** * Flat mapping: definition and lemmas *)
+
+(* a propositional version of flat_map *)
+(* FlatMap lbase f lmapped means that lmapped corresponds to the list lbase where each element has been replaced by its image by f *)
+Inductive FlatMap {X Y:Type} : list X -> (X -> list Y -> Prop) -> list Y -> Prop :=
+| FM_nil: forall f,
+  FlatMap [] f []
+| FM_cons:
+  forall lbase f lmapped x ly
+    (FM: FlatMap lbase f lmapped)
+    (HEAD: f x ly),
+    FlatMap (x::lbase) f (ly ++ lmapped).
+
+(* We could use the functional flat_map, but this would require using the function compute_tr that associates a tree to each regex and input. *)
+(* The proof does not strictly rely on this function, it merely relies on the
+existence of a unique tree associated to each regex and input. *)
+
+(* Used in disjunction and free quantifier cases of contextual equivalence proof *)
+Property FlatMap_app {X Y: Type}:
+  forall (lbase1 lbase2 : list X) (f: X -> list Y -> Prop) (lmapped1 lmapped2: list Y),
+    FlatMap lbase1 f lmapped1 ->
+    FlatMap lbase2 f lmapped2 ->
+    FlatMap (lbase1 ++ lbase2) f (lmapped1 ++ lmapped2).
+Proof.
+  intros lbase1 lbase2 f lmapped1 lmapped2 FM1 FM2.
+  induction FM1.
+  - auto.
+  - rewrite <- app_assoc, <- app_comm_cons. constructor; auto.
+Qed.
+
+(* Determinism of a propositional function *)
+Definition determ {A B: Type} (f: A -> B -> Prop) :=
+  forall x y1 y2, f x y1 -> f x y2 -> y1 = y2.
+
+
+(* Building up to flatmap_leaves_equiv_l *)
+
+Lemma FlatMap_in {A B}:
+  forall (l: list A) (f: A -> list B -> Prop) fl x fx,
+    (* For a deterministic f, *)
+    determ f ->
+    (* if f flat maps l to fl, *)
+    FlatMap l f fl ->
+    (* and x is in l, *)
+    In x l ->
+    f x fx ->
+    (* then all the elements of f(x) are in fl. *)
+    Forall (fun y => In y fl) fx.
+Proof.
+  intros l f fl x fx DETERM FM INxl F.
+  revert fl FM.
+  induction l.
+  1: inversion INxl.
+  intros fl FM. destruct INxl.
+  - subst a. inversion FM; subst.
+    assert (ly = fx) by eauto (* using DETERM *). subst ly. clear HEAD FM F IHl.
+    induction fx.
+    + constructor.
+    + constructor.
+      * rewrite <- app_comm_cons. left. reflexivity.
+      * eapply Forall_impl; eauto. simpl. tauto.
+  - inversion FM; subst. specialize (IHl H lmapped FM0).
+    eapply Forall_impl; eauto. simpl. intro. rewrite in_app_iff. tauto.
+Qed.
+
+Section Leaves.
+  Context {params: LindenParameters}.
+  Context (rer: RegExpRecord).
+
+(* Getting the leaves of a continuation applied to a particular leaf *)
+(* This predicate will be used to express that appending a list of actions a2 to a list
+of actions a1 corresponds to extending the leaves of the tree corresponding to actions
+a1 with trees corresponding to the actions of a2 (see lemma leaves_concat below) *)
+Inductive act_from_leaf : actions -> Direction -> leaf -> list leaf -> Prop :=
+| afl:
+  forall act dir l t
+    (TREE: is_tree rer act (fst l) (snd l) dir t),
+    act_from_leaf act dir l (tree_leaves t (snd l) (fst l) dir).
+
+(* The function act_from_leaf is deterministic *)
+Lemma act_from_leaf_determ: forall act dir, determ (act_from_leaf act dir).
+Proof.
+  intros act dir x y1 y2 Hxy1 Hxy2.
+  inversion Hxy1; subst. inversion Hxy2; subst.
+  assert (t0 = t) by eauto using is_tree_determ. subst t0. reflexivity.
+Qed.
+
+(* Adding new things to the continuation is the same as extending each leaf of the tree with these new things *)
+Theorem leaves_concat:
+  forall inp gm dir act1 act2 tapp t1
+    (TREE_APP: is_tree rer (act1 ++ act2) inp gm dir tapp)
+    (TREE_1: is_tree rer act1 inp gm dir t1),
+    FlatMap (tree_leaves t1 gm inp dir) (act_from_leaf act2 dir) (tree_leaves tapp gm inp dir).
+Proof.
+  intros. generalize dependent tapp.
+  induction TREE_1; intros; simpl in *.
+  - (* Done *)
+    rewrite <- app_nil_r. constructor; constructor. auto.
+
+  - (* Check pass *)
+    inversion TREE_APP; subst. 2: contradiction.
+    simpl. apply IHTREE_1. auto.
+
+  - (* Check fail *)
+    inversion TREE_APP; subst. 1: contradiction.
+    simpl. constructor.
+
+  - (* Close *)
+    inversion TREE_APP; subst. simpl.
+    apply IHTREE_1. auto.
+
+  - (* Epsilon *)
+    inversion TREE_APP; subst. auto.
+
+  - (* Read char success *)
+    inversion TREE_APP; subst. 2: congruence.
+    simpl.
+    rewrite READ in READ0. injection READ0 as <- <-.
+    rewrite advance_input_success with (nexti := nextinp).
+    2: eauto using read_char_success_advance.
+    auto.
+
+  - (* Read char fail *)
+    inversion TREE_APP; subst. 1: congruence.
+    simpl. constructor.
+
+  - (* Disjunction *)
+    inversion TREE_APP; subst.
+    simpl. apply FlatMap_app; auto.
+
+  - (* Sequence *)
+    inversion TREE_APP; subst.
+    rewrite app_assoc in CONT. auto.
+
+  - (* Forced quantifier *)
+    inversion TREE_APP; subst. simpl.
+    auto.
+
+  - (* Done quantifier *)
+    inversion TREE_APP; subst.
+    2: { destruct plus; discriminate. }
+    auto.
+
+  - (* Free quantifier *)
+    inversion TREE_APP; subst.
+    1: { destruct plus; discriminate. }
+    assert (plus0 = plus). {
+      destruct plus0; destruct plus; try discriminate; try reflexivity.
+      injection H1 as <-. auto.
+    }
+    subst plus0.
+    unfold greedy_choice. destruct greedy.
+    + (* Greedy *)
+      simpl. apply FlatMap_app; auto.
+    + (* Lazy *)
+      simpl. apply FlatMap_app; auto.
+
+  - (* Group *)
+    inversion TREE_APP; subst. simpl.
+    auto.
+
+  - (* Lookaround success *)
+    inversion TREE_APP; subst;
+      assert (treelk0 = treelk) by (eapply is_tree_determ; eauto); subst.
+    2: { rewrite RES_LK in FAIL_LK. inversion FAIL_LK. }
+    rewrite RES_LK in RES_LK0. injection RES_LK0 as <-.
+    destruct positivity eqn:Hpos.
+    + unfold lk_result in RES_LK. rewrite Hpos in RES_LK.
+      pose proof first_tree_leaf treelk gm inp (lk_dir lk) as LK_FIRST.
+      destruct (tree_res treelk gm inp (lk_dir lk)) as [[inplk gmlk']|] eqn:TREERES_LK; try discriminate.
+      injection RES_LK as ->.
+      destruct (tree_leaves treelk gm inp (lk_dir lk)) as [|[inplk' gmlk'] q] eqn:TREELEAVES_LK; try discriminate.
+      simpl in *. injection LK_FIRST as <- <-. rewrite Hpos.
+      rewrite TREELEAVES_LK. auto.
+    + unfold lk_result in RES_LK. rewrite Hpos in RES_LK.
+      destruct (tree_res treelk gm inp (lk_dir lk)) eqn:TREERES; inversion RES_LK. subst.
+      assert (tree_leaves treelk gmlk inp (lk_dir lk) = []).
+      { apply leaves_indep with (gm1 := gmlk) (inp1 := inp) (dir1 := lk_dir lk).
+        apply hd_error_none_nil. rewrite <- first_tree_leaf. auto. }
+      simpl. rewrite Hpos, H. auto.
+
+  - (* Lookaround failure *)
+    inversion TREE_APP; subst;
+      assert (treelk0 = treelk) by (eapply is_tree_determ; eauto); subst.
+    { rewrite RES_LK in FAIL_LK. inversion FAIL_LK. }
+    simpl. constructor.
+
+  - (* Anchor *)
+    inversion TREE_APP; subst.
+    2: congruence.
+    simpl. auto.
+
+  - (* Anchor fail *)
+    inversion TREE_APP; subst.
+    1: congruence.
+    simpl. constructor.
+
+  - (* Backref *)
+    inversion TREE_APP; subst.
+    2: congruence.
+    rewrite READ_BACKREF in READ_BACKREF0. injection READ_BACKREF0 as <- <-.
+    simpl.
+    replace (advance_input_n _ _ _) with nextinp.
+    2: eauto using read_backref_success_advance.
+    auto.
+
+  - (* Backref fail *)
+    inversion TREE_APP; subst.
+    1: congruence.
+    simpl. constructor.
+Qed.
+
+End Leaves.
